Re-engineer prompt monad of Lem shallow embedding
- Use simplified monad type (e.g., without the with_aux constructors that are
  not needed by the shallow embedding).
- Add support for registers with arbitrary types (e.g., records, enumerations,
  vectors of vectors). Instead of using bit lists as the common representation
  of register values at the monad interface, use a register_value type that is
  generated per spec as a union of all register types that occur in the spec.
  Conversion functions between register_value and concrete types are generated.
- Use the same representation of register references as the state monad, in
  preparation of rebasing the state monad onto the prompt monad.
- Split out those types from sail_impl_base.lem that are used by the shallow
  embedding into a new module sail_instr_kinds.lem, and import that.  Removing
  the dependency on Sail_impl_base from the shallow embedding avoids name clashes
  between the different monad types.

Not yet done:
- Support for reading/writing register slices.  Currently, a rewriting pass
  pushes register slices in l-expressions to the right-hand side, turning a
  write to a register slice into a read-modify-write.  For interfacing with the
  concurreny model, we will want to be more precise than that (in particular
  since some specs represent register files as big single registers containing a
  vector of bitvectors).
- Lemmas about the conversion functions to/from register_value should be
  generated automatically.

src/ast_util.ml
@@ -712,6 +712,21 @@ let rec string_of_index_range (BF_aux (ir, _)) =
   | BF_range (n, m) -> Big_int.to_string n ^ " .. " ^ Big_int.to_string m
   | BF_concat (ir1, ir2) -> "(" ^ string_of_index_range ir1 ^ ") : (" ^ string_of_index_range ir2 ^ ")"
 
+
+let rec pat_ids (P_aux (pat_aux, _)) =
+  match pat_aux with
+  | P_lit _ | P_wild -> IdSet.empty
+  | P_id id -> IdSet.singleton id
+  | P_as (pat, id) -> IdSet.add id (pat_ids pat)
+  | P_var (pat, _) | P_typ (_, pat) -> pat_ids pat
+  | P_app (_, pats) | P_tup pats | P_vector pats | P_vector_concat pats | P_list pats ->
+     List.fold_right IdSet.union (List.map pat_ids pats) IdSet.empty
+  | P_cons (pat1, pat2) ->
+     IdSet.union (pat_ids pat1) (pat_ids pat2)
+  | P_record (fpats, _) ->
+     List.fold_right IdSet.union (List.map fpat_ids fpats) IdSet.empty
+and fpat_ids (FP_aux (FP_Fpat (_, pat), _)) = pat_ids pat
+
 let id_of_fundef (FD_aux (FD_function (_, _, _, funcls), (l, _))) =
   match (List.fold_right
            (fun (FCL_aux (FCL_Funcl (id, _), _)) id' ->
@@ -732,6 +747,20 @@ let id_of_type_def_aux = function
   | TD_enum (id, _, _, _)
   | TD_bitfield (id, _, _) -> id
 let id_of_type_def (TD_aux (td_aux, _)) = id_of_type_def_aux td_aux
+
+let id_of_val_spec (VS_aux (VS_val_spec (_, id, _, _), _)) = id
+
+let ids_of_def = function
+  | DEF_kind (KD_aux (KD_nabbrev (_, id, _, _), _)) -> IdSet.singleton id
+  | DEF_type td -> IdSet.singleton (id_of_type_def td)
+  | DEF_fundef fd -> IdSet.singleton (id_of_fundef fd)
+  | DEF_val (LB_aux (LB_val (pat, _), _)) -> pat_ids pat
+  | DEF_reg_dec (DEC_aux (DEC_reg (_, id), _)) -> IdSet.singleton id
+  | DEF_spec vs -> IdSet.singleton (id_of_val_spec vs)
+  | DEF_internal_mutrec fds -> IdSet.of_list (List.map id_of_fundef fds)
+  | _ -> IdSet.empty
+let ids_of_defs (Defs defs) =
+  List.fold_left IdSet.union IdSet.empty (List.map ids_of_def defs)
 
 module BE = struct
   type t = base_effect
@@ -965,25 +994,12 @@ let split_defs f (Defs defs) =
      Some (Defs (List.rev pre_defs), def, Defs post_defs)
 
 let append_ast (Defs ast1) (Defs ast2) = Defs (ast1 @ ast2)
+let concat_ast asts = List.fold_right append_ast asts (Defs [])
 
 let type_union_id (Tu_aux (aux, _)) = match aux with
   | Tu_id id -> id
   | Tu_ty_id (_, id) -> id
 
-
-let rec pat_ids (P_aux (pat_aux, _)) =
-  match pat_aux with
-  | P_lit _ | P_wild -> IdSet.empty
-  | P_id id -> IdSet.singleton id
-  | P_as (pat, id) -> IdSet.add id (pat_ids pat)
-  | P_var (pat, _) | P_typ (_, pat) -> pat_ids pat
-  | P_app (_, pats) | P_tup pats | P_vector pats | P_vector_concat pats | P_list pats ->
-     List.fold_right IdSet.union (List.map pat_ids pats) IdSet.empty
-  | P_cons (pat1, pat2) ->
-     IdSet.union (pat_ids pat1) (pat_ids pat2)
-  | P_record (fpats, _) ->
-     List.fold_right IdSet.union (List.map fpat_ids fpats) IdSet.empty
-and fpat_ids (FP_aux (FP_Fpat (_, pat), _)) = pat_ids pat
 
 let rec subst id value (E_aux (e_aux, annot) as exp) =
   let wrap e_aux = E_aux (e_aux, annot) in
