src/state.ml
@@ -1,0 +1,279 @@
+(**************************************************************************)
+(*     Sail                                                               *)
+(*                                                                        *)
+(*  Copyright (c) 2013-2017                                               *)
+(*    Kathyrn Gray                                                        *)
+(*    Shaked Flur                                                         *)
+(*    Stephen Kell                                                        *)
+(*    Gabriel Kerneis                                                     *)
+(*    Robert Norton-Wright                                                *)
+(*    Christopher Pulte                                                   *)
+(*    Peter Sewell                                                        *)
+(*    Alasdair Armstrong                                                  *)
+(*    Brian Campbell                                                      *)
+(*    Thomas Bauereiss                                                    *)
+(*    Anthony Fox                                                         *)
+(*    Jon French                                                          *)
+(*    Dominic Mulligan                                                    *)
+(*    Stephen Kell                                                        *)
+(*    Mark Wassell                                                        *)
+(*                                                                        *)
+(*  All rights reserved.                                                  *)
+(*                                                                        *)
+(*  This software was developed by the University of Cambridge Computer   *)
+(*  Laboratory as part of the Rigorous Engineering of Mainstream Systems  *)
+(*  (REMS) project, funded by EPSRC grant EP/K008528/1.                   *)
+(*                                                                        *)
+(*  Redistribution and use in source and binary forms, with or without    *)
+(*  modification, are permitted provided that the following conditions    *)
+(*  are met:                                                              *)
+(*  1. Redistributions of source code must retain the above copyright     *)
+(*     notice, this list of conditions and the following disclaimer.      *)
+(*  2. Redistributions in binary form must reproduce the above copyright  *)
+(*     notice, this list of conditions and the following disclaimer in    *)
+(*     the documentation and/or other materials provided with the         *)
+(*     distribution.                                                      *)
+(*                                                                        *)
+(*  THIS SOFTWARE IS PROVIDED BY THE AUTHOR AND CONTRIBUTORS ``AS IS''    *)
+(*  AND ANY EXPRESS OR IMPLIED WARRANTIES, INCLUDING, BUT NOT LIMITED     *)
+(*  TO, THE IMPLIED WARRANTIES OF MERCHANTABILITY AND FITNESS FOR A       *)
+(*  PARTICULAR PURPOSE ARE DISCLAIMED.  IN NO EVENT SHALL THE AUTHOR OR   *)
+(*  CONTRIBUTORS BE LIABLE FOR ANY DIRECT, INDIRECT, INCIDENTAL,          *)
+(*  SPECIAL, EXEMPLARY, OR CONSEQUENTIAL DAMAGES (INCLUDING, BUT NOT      *)
+(*  LIMITED TO, PROCUREMENT OF SUBSTITUTE GOODS OR SERVICES; LOSS OF      *)
+(*  USE, DATA, OR PROFITS; OR BUSINESS INTERRUPTION) HOWEVER CAUSED AND   *)
+(*  ON ANY THEORY OF LIABILITY, WHETHER IN CONTRACT, STRICT LIABILITY,    *)
+(*  OR TORT (INCLUDING NEGLIGENCE OR OTHERWISE) ARISING IN ANY WAY OUT    *)
+(*  OF THE USE OF THIS SOFTWARE, EVEN IF ADVISED OF THE POSSIBILITY OF    *)
+(*  SUCH DAMAGE.                                                          *)
+(**************************************************************************)
+
+module Big_int = Nat_big_num
+
+open Initial_check
+open Type_check
+open Ast
+open Ast_util
+open PPrint
+open Pretty_print_common
+open Pretty_print_sail
+
+let defs_of_string = ast_of_def_string Ast_util.inc_ord
+
+let find_registers defs =
+  List.fold_left
+    (fun acc def ->
+      match def with
+      | DEF_reg_dec (DEC_aux(DEC_reg (typ, id), annot)) ->
+         let env = match annot with
+           | (_, Some (env, _, _)) -> env
+           | _ -> Env.empty
+         in
+         (Env.expand_synonyms env typ, id) :: acc
+      | _ -> acc
+    ) [] defs
+
+let generate_regstate = function
+  | [] -> ["type regstate = unit"]
+  | registers ->
+     let reg (typ, id) = Printf.sprintf "%s : %s" (string_of_id id) (to_string (doc_typ typ)) in
+     let initreg (_, id) = Printf.sprintf "%s = undefined" (string_of_id id) in
+     let regstate =
+       "struct regstate = { " ^
+       (String.concat ", " (List.map reg registers)) ^
+       " }"
+     in
+     let initstate =
+       "let initial_regstate : regstate = struct { " ^
+       (String.concat ", " (List.map initreg registers)) ^
+       " }"
+     in
+     regstate :: (if !Initial_check.opt_undefined_gen then [initstate] else [])
+
+let rec regval_constr_id mwords (Typ_aux (t, l) as typ) = match t with
+  | Typ_id id -> id
+  | Typ_app (id, args) ->
+     let name_arg (Typ_arg_aux (targ, _)) = match targ with
+       | Typ_arg_typ targ -> string_of_id (regval_constr_id mwords targ)
+       | Typ_arg_nexp nexp when is_nexp_constant (nexp_simp nexp) ->
+          string_of_nexp (nexp_simp nexp)
+       | Typ_arg_order (Ord_aux (Ord_inc, _)) -> "inc"
+       | Typ_arg_order (Ord_aux (Ord_dec, _)) -> "dec"
+       | _ ->
+          raise (Reporting_basic.err_typ l "Unsupported register type")
+     in
+     let builtins = IdSet.of_list (List.map mk_id ["vector"; "list"; "option"]) in
+     if IdSet.mem id builtins && not (mwords && is_bitvector_typ typ) then id else
+     append_id id (String.concat "_" ("" :: List.map name_arg args))
+  | _ -> raise (Reporting_basic.err_typ l "Unsupported register type")
+
+let register_base_types mwords typs =
+  let rec add_base_typs typs (Typ_aux (t, _) as typ) =
+    let builtins = IdSet.of_list (List.map mk_id ["vector"; "list"; "option"]) in
+    match t with
+      | Typ_app (id, args)
+        when IdSet.mem id builtins && not (mwords && is_bitvector_typ typ) ->
+         let add_typ_arg base_typs (Typ_arg_aux (targ, _)) =
+           match targ with
+             | Typ_arg_typ typ -> add_base_typs typs typ
+             | _ -> typs
+         in
+         List.fold_left add_typ_arg typs args
+      | _ -> Bindings.add (regval_constr_id mwords typ) typ typs
+  in
+  List.fold_left add_base_typs Bindings.empty typs
+
+let generate_regval_typ typs =
+  let constr (constr_id, typ) =
+    Printf.sprintf "Regval_%s : %s" (string_of_id constr_id) (to_string (doc_typ typ)) in
+  let builtins =
+    "Regval_vector : (int, bool, list(register_value)), " ^
+    "Regval_list : list(register_value), " ^
+    "Regval_option : option(register_value)"
+  in
+  ["union register_value = { " ^
+  (String.concat ", " (builtins :: List.map constr (Bindings.bindings typs))) ^
+  " }"]
+
+let add_regval_conv id typ defs =
+  let id = string_of_id id in
+  let is_defined name = IdSet.mem (mk_id name) (ids_of_defs defs) in
+  let typ_str = to_string (doc_typ typ) in
+  (* Create a function that converts from regval to the target type. *)
+  let from_name = id ^ "_of_regval" in
+  let from_val = Printf.sprintf "val %s : register_value -> option(%s)" from_name typ_str in
+  let from_function = String.concat "\n" [
+    Printf.sprintf "function %s Regval_%s(v) = Some(v)" from_name id;
+    Printf.sprintf "and %s _ = None" from_name
+    ] in
+  let from_defs = if is_defined from_name then [] else [from_val; from_function] in
+  (* Create a function that converts from target type to regval. *)
+  let to_name = "regval_of_" ^ id in
+  let to_val = Printf.sprintf "val %s : %s -> register_value" to_name typ_str in
+  let to_function = Printf.sprintf "function %s v = Regval_%s(v)" to_name id in
+  let to_defs = if is_defined to_name then [] else [to_val; to_function] in
+  let cdefs = concat_ast (List.map defs_of_string (from_defs @ to_defs)) in
+  append_ast defs cdefs
+
+let rec regval_convs_lem mwords (Typ_aux (t, _) as typ) = match t with
+  | Typ_app _ when is_vector_typ typ && not (mwords && is_bitvector_typ typ) ->
+     let _, size, ord, etyp = vector_typ_args_of typ in
+     let size = string_of_nexp (nexp_simp size) in
+     let is_inc = if is_order_inc ord then "true" else "false" in
+     let etyp_of, of_etyp = regval_convs_lem mwords etyp in
+     "(fun v -> vector_of_regval " ^ etyp_of ^ " v)",
+     "(fun v -> regval_of_vector " ^ of_etyp ^ " " ^ size ^ " " ^ is_inc ^ " v)"
+  | Typ_app (id, [Typ_arg_aux (Typ_arg_typ etyp, _)])
+    when string_of_id id = "list" ->
+     let etyp_of, of_etyp = regval_convs_lem mwords etyp in
+     "(fun v -> list_of_regval " ^ etyp_of ^ " v)",
+     "(fun v -> regval_of_list " ^ of_etyp ^ " v)"
+  | Typ_app (id, [Typ_arg_aux (Typ_arg_typ etyp, _)])
+    when string_of_id id = "option" ->
+     let etyp_of, of_etyp = regval_convs_lem mwords etyp in
+     "(fun v -> option_of_regval " ^ etyp_of ^ " v)",
+     "(fun v -> regval_of_option " ^ of_etyp ^ " v)"
+  | _ ->
+     let id = string_of_id (regval_constr_id mwords typ) in
+     "(fun v -> " ^ id ^ "_of_regval v)", "(fun v -> regval_of_" ^ id ^ " v)"
+
+let register_refs_lem prefix_recordtype mwords registers =
+  let generic_convs =
+    separate_map hardline string [
+      "val vector_of_regval : forall 'a. (register_value -> maybe 'a) -> register_value -> maybe (list 'a)";
+      "let vector_of_regval of_regval = function";
+      "  | Regval_vector (_, _, v) -> just_list (List.map of_regval v)";
+      "  | _ -> Nothing";
+      "end";
+      "";
+      "val regval_of_vector : forall 'a. ('a -> register_value) -> integer -> bool -> list 'a -> register_value";
+      "let regval_of_vector regval_of size is_inc xs = Regval_vector (size, is_inc, List.map regval_of xs)";
+      "";
+      "val list_of_regval : forall 'a. (register_value -> maybe 'a) -> register_value -> maybe (list 'a)";
+      "let list_of_regval of_regval = function";
+      "  | Regval_list v -> just_list (List.map of_regval v)";
+      "  | _ -> Nothing";
+      "end";
+      "";
+      "val regval_of_list : forall 'a. ('a -> register_value) -> list 'a -> register_value";
+      "let regval_of_list regval_of xs = Regval_list (List.map regval_of xs)";
+      "";
+      "val option_of_regval : forall 'a. (register_value -> maybe 'a) -> register_value -> maybe (maybe 'a)";
+      "let option_of_regval of_regval = function";
+      "  | Regval_option v -> Maybe.map of_regval v";
+      "  | _ -> Nothing";
+      "end";
+      "";
+      "val regval_of_option : forall 'a. ('a -> register_value) -> maybe 'a -> register_value";
+      "let regval_of_option regval_of v = Regval_option (Maybe.map regval_of v)";
+      "";
+      ""
+    ]
+  in
+  let register_ref (typ, id) =
+    let idd = string (string_of_id id) in
+    let field = if prefix_recordtype then string "regstate_" ^^ idd else idd in
+    let is_inc =
+      if is_bitvector_typ typ then
+        let _, _, ord, _ = vector_typ_args_of typ in
+        if is_order_inc ord then "true" else "false"
+      else "true"
+    in
+    let of_regval, regval_of = regval_convs_lem mwords typ in
+    concat [string "let "; idd; string " = <|"; hardline;
+      string "  name = \""; idd; string "\";"; hardline;
+      string "  is_inc = "; string is_inc; string ";"; hardline;
+      string "  read_from = (fun s -> s."; field; string ");"; hardline;
+      string "  write_to = (fun s v -> (<| s with "; field; string " = v |>));"; hardline;
+      string "  of_regval = "; string of_regval; string ";"; hardline;
+      string "  regval_of = "; string regval_of; string " |>"; hardline]
+  in
+  let refs = separate_map hardline register_ref registers in
+  let get_set_reg (_, id) =
+    let idd = string_of_id id in
+    string ("  if reg_name = \"" ^ idd ^ "\" then Just (" ^ idd ^ ".regval_of (" ^ idd ^ ".read_from s)) else"),
+    string ("  if reg_name = \"" ^ idd ^ "\" then Maybe.map (" ^ idd ^ ".write_to s) (" ^ idd ^ ".of_regval v) else")
+  in
+  let getters_setters =
+    let getters, setters = List.split (List.map get_set_reg registers) in
+    string "val get_regval : string -> regstate -> maybe register_value" ^^ hardline ^^
+    string "let get_regval reg_name s =" ^^ hardline ^^
+    separate hardline getters ^^ hardline ^^
+    string "  Nothing" ^^ hardline ^^ hardline ^^
+    string "val set_regval : string -> register_value -> regstate -> maybe regstate" ^^ hardline ^^
+    string "let set_regval reg_name v s =" ^^ hardline ^^
+    separate hardline setters ^^ hardline ^^
+    string "  Nothing" ^^ hardline ^^ hardline ^^
+    string "let register_accessors = (get_regval, set_regval)" ^^ hardline ^^ hardline
+  in
+  separate hardline [generic_convs; refs; getters_setters]
+
+let generate_regstate_defs mwords defs =
+  let registers = find_registers defs in
+  let def_ids = ids_of_defs (Defs defs) in
+  let has_def name = IdSet.mem (mk_id name) def_ids in
+  let regtyps = register_base_types mwords (List.map fst registers) in
+  let option_typ =
+    if has_def "option" then [] else
+      ["union option ('a : Type) = {None, Some : 'a}"]
+  in
+  let regval_typ = if has_def "register_value" then [] else generate_regval_typ regtyps in
+  let regstate_typ = if has_def "regstate" then [] else generate_regstate registers in
+  (* FIXME We currently don't want to generate undefined_type functions
+     for register state and values.  For the Lem backend, this would require
+     taking the dependencies of those functions into account when partitioning
+     definitions into the different lem files, which we currently don't do. *)
+  let gen_undef = !Initial_check.opt_undefined_gen in
+  Initial_check.opt_undefined_gen := false;
+  let defs =
+    option_typ @ regval_typ @ regstate_typ
+    |> List.map defs_of_string
+    |> concat_ast
+    |> Bindings.fold add_regval_conv regtyps
+  in
+  Initial_check.opt_undefined_gen := gen_undef;
+  defs
+
+let add_regstate_defs mwords env (Defs defs) =
+  let reg_defs, env = check env (generate_regstate_defs mwords defs) in
+  env, append_ast (Defs defs) reg_defs
